src/Lean/Elab/Tactic/Do/ProofMode/Exfalso.lean
@@ -15,8 +15,8 @@ open Lean Elab Tactic Meta
 
 -- set_option pp.all true in
 -- #check ⌜False⌝
-private def falseProp (σs : Expr) : Expr := -- ⌜False⌝ standing in for an empty conjunction of hypotheses
-  mkApp3 (mkConst ``SVal.curry) (.sort .zero) σs <| mkLambda `escape .default (mkApp (mkConst ``SVal.StateTuple) σs) (mkConst ``False)
+private def falseProp (u : Level) (σs : Expr) : Expr := -- ⌜False⌝ standing in for an empty conjunction of hypotheses
+  mkApp3 (mkConst ``SVal.curry [u]) (mkApp (mkConst ``ULift [u, 0]) (.sort .zero)) σs <| mkLambda `tuple .default (mkApp (mkConst ``SVal.StateTuple [u]) σs) (mkApp2 (mkConst ``ULift.up [u, 0]) (.sort .zero) (mkConst ``False))
 
 @[builtin_tactic Lean.Parser.Tactic.mexfalso]
 def elabMExfalso : Tactic | _ => do
@@ -24,8 +24,8 @@ def elabMExfalso : Tactic | _ => do
   mvar.withContext do
   let g ← instantiateMVars <| ← mvar.getType
   let some goal := parseMGoal? g | throwError "not in proof mode"
-  let newGoal := { goal with target := falseProp goal.σs }
+  let newGoal := { goal with target := falseProp goal.u goal.σs }
   let m ← mkFreshExprSyntheticOpaqueMVar newGoal.toExpr
-  let prf := mkApp4 (mkConst ``SPred.exfalso) goal.σs goal.hyps goal.target m
+  let prf := mkApp4 (mkConst ``SPred.exfalso [goal.u]) goal.σs goal.hyps goal.target m
   mvar.assign prf
   replaceMainGoal [m.mvarId!]
